cleaned version - all 3 theorems

work.v
@@ -1,32 +1,12 @@
-
-
-(** * Adapting to CPOs *)
-
 From Coq Require Import Arith.
 Require Import Psatz.
 Require Export Setoid Morphisms.
 Set Implicit Arguments.
 
-(*
-Definition even_type : Type := {n:nat | Arith.Even.even n}.
-Lemma is_not_odd (n:even_type) : ~ Arith.Even.odd (proj1_sig n).
-Proof.
-  destruct n. cbn. intuition.
-Admitted.
-*)
 
-(*
-Definition Directed_generalized X (D:X->Prop) (leq : relation X) := 
-  forall x y, D x -> D y -> exists z, D z /\ leq x z /\ leq y z.
-Definition directed_set_generalized X (Directed : (X -> Prop) -> Prop) : Type :=
-  {Dbody : X -> Prop | Directed Dbody}.
-Definition Dbody_generalized X P (D:sig P) : X -> Prop :=
-  proj1_sig D.
-*)
+(* Definition of Directed sets for some order relation <=. D is directed if :
+forall x y in D, there is a z in D such that x <= z and y <= z. *)
 
-(* First we define what are directed sets.
-    Here I do it completely naïvely, taking as argument the minimal needed. We could imagine also defining posets (or taking the def from the standard library), define directed sets over posets, and cpo as specific posets
- *)
 Notation set X := (X -> Prop).
 Notation rel X := (X -> X -> Prop).
 Definition Directed {X} `(leq : rel X) (D : set X) : Prop :=
@@ -34,7 +14,7 @@ Definition Directed {X} `(leq : rel X) (D : set X) : Prop :=
 Definition directed_set {X} (leq : rel X) := {Dbody : set X | Directed leq Dbody}.
 Definition Dbody {X leq} (D : directed_set leq) : set X := proj1_sig D.
 
-(* Here we have the same fields as before, but we now call definitions that are not functions of CPO, but simply of operations that CPOs happen to have *)
+(* Definition of a CPO : Complete Partially Ordered set, and Lattice as a particular (stronger) CPO. *)
 Class CPO (X: Type) := {
   weq: relation X;
   leq: relation X;
@@ -42,71 +22,18 @@ Class CPO (X: Type) := {
   PreOrder_leq:> PreOrder leq;
   weq_spec: forall x y, weq x y <-> (leq x y /\ leq y x);
   sup_spec: forall D z, (leq (sup D) z <-> forall (y:X), (Dbody D) y -> leq y z);
-  }.
-
-Definition reverse_leq X (leq : X -> X -> Prop) : X -> X -> Prop := fun x y => leq y x.
-
-(* And now this work: notice that I pass `reverse_leq` to `Dbody` in the definition of `sup`.
-   If I am not mistaken that corresponds to what you were looking for, but I mostly followed the types without thinking of the semantics so I might be off :)
- *)
-(*
-Global Program Instance reverse_CPO X (P: CPO X): CPO X := {|
-   weq := weq;
-   leq := reverse_leq leq;
-   sup D := sup (fun z => forall y, (@Dbody _ (reverse_leq leq) D y) -> leq z y);
- |}.
- *)
- 
-(* Old versions *)
-(*
-Class CPO (X: Type) := {
-  weq: relation X;
-  leq: relation X;
-  Directed (D: X -> Prop) := forall x y, D x -> D y -> exists z, D z /\ leq x z /\ leq y z;
-  directed_set : Type := {Dbody : X -> Prop | Directed Dbody};
-  Dbody (D:directed_set) : X -> Prop :=  proj1_sig D;
-  sup: directed_set -> X;
-  PreOrder_leq:> PreOrder leq;
-  weq_spec: forall x y, weq x y <-> (leq x y /\ leq y x);
-  sup_spec: forall D z, (leq (sup D) z <-> forall (y:X), (Dbody D) y -> leq y z);
-                        }.
-
-Class CPO (X: Type) := {
-  weq: relation X;
-  leq: relation X;
-  sup: (X -> Prop) -> X -> Prop;
-  PreOrder_leq:> PreOrder leq;
-  Directed (D: X -> Prop) := forall x y, D x -> D y -> exists z, D z /\ leq x z /\ leq y z;
-  weq_spec: forall x y, weq x y <-> (leq x y /\ leq y x);
-  sup_spec: forall D s, sup D s -> forall z, (leq s z <-> forall y, D y -> leq y z);
-  sup_exists: forall D, Directed D -> exists s, sup D s;
-  (*sup_spec: forall Y z, Directed Y ->  (leq (sup Y) z <-> forall y, Y y -> leq y z);*)
-                        }.*)
+}.
 
 Class CompleteLattice (X : Type) `(L : CPO X) := {
     sup_lat: (X -> Prop) -> X;
     sup_spec_lat:  forall Y z, (leq (sup_lat Y) z <-> forall y, Y y -> leq y z);
-                                  }.
-Declare Scope CPO.
+}.
+
+Declare Scope CPO. (* I don't really understand there 2 lines. *)
 Open Scope CPO.
 Infix "==" := weq (at level 70): CPO.
 Infix "<=" := leq: CPO.
 Global Hint Extern 0 => reflexivity: core.
-
-(** * Reversing a CPO *)
-
-(*Bad Idea, don't actually do it... *)
-(*
-Definition reverse_leq X (leq : X -> X -> Prop) : X -> X -> Prop := fun x y => leq y x.
-
-Global Program Instance reverse_CPO (P: CPO X): CPO X := {|
-   weq := weq;
-   leq := reverse_leq leq;
-   sup D := sup (fun z => forall y, (@Dbody X (reverse_CPO X) D y) -> leq z y); 
-   (*Careful ! I dunno which "leq" is used here :/*)
- |}.
- Next Obligation.
-*)
 
 (** * Utilities  *)
 
@@ -122,40 +49,72 @@ Proof.
   apply weq_spec. split; apply Hf; (apply E || apply E').
 Qed.
 
-(** * General properties*)
 
-Section sup.
- Context {X} {P Q: CPO X} `{L : CompleteLattice X}.
- 
- (*Below lemma is necessary for later property.*)
- Lemma directed_symmetry f g : (forall z, f z <-> g z) -> Directed leq f <-> Directed leq g.
+(** * Sets general properties *)
+
+Section Sets.
+
+ Context {X} {P: CPO X}.
+
+ Definition iff_part (f g : X -> Prop) := forall z, f z <-> g z. (*equality of sets*)
+
+ Definition included (S T: set X) := forall x, S x -> T x.
+
+ #[global] Instance Included_trans : Transitive included.
  Proof.
-  intro H. unfold Directed. (* unfold Directed_generalized. *)setoid_rewrite H. tauto.
-Qed.
+  intros Y1 Y2 Y3 H12 H13. intros x H. apply H13. now apply H12.
+ Qed.
 
-Definition iff_part (f g : X -> Prop) := forall z, f z <-> g z.
-Locate "<->".
-Global Instance directed_eq : Proper (iff_part ==> iff) (Directed leq).
-Proof. intros f g. apply directed_symmetry. Qed.
+End Sets.
+Infix "⊆" := included (at level 70).
 
-Lemma singleton_is_directed x : Directed leq (fun z => z=x).
+
+(** * Directedness general properties *)
+
+Section Directedness.
+
+ Context {X} {P: CPO X}.
+
+ Lemma directed_symmetry f g : (forall z, f z <-> g z) -> Directed leq f <-> Directed leq g.
+ Proof. intro H. unfold Directed. setoid_rewrite H. tauto. Qed.
+
+ #[global] Instance directed_eq : Proper (iff_part ==> iff) (Directed leq).
+ Proof. intros f g. apply directed_symmetry. Qed.
+
+ Lemma singleton_is_directed x : Directed leq (fun z => z=x).
+ Proof. unfold Directed. intros y z Hyz. exists x. repeat split. now rewrite Hyz. now rewrite H. Qed.
+
+Definition is_Chain (Y : set X) := forall (x y : X), Y x -> Y y -> x <= y \/ y <= x.
+
+Lemma chain_is_directed {Y} {Q : CPO Y} : forall D, is_Chain D -> Directed leq D.
 Proof.
-  unfold Directed. intros. exists x. repeat split. now rewrite H. now rewrite H0.
+  intros D Hd x y Hx Hy. destruct (Hd x y); intuition.
+  exists y. now split.
+  exists x. now split.
 Qed.
 
 
- (** Partial order *)
- Global Instance Equivalence_weq: Equivalence weq.
+End Directedness.
+
+(** Partial Order general properties *)
+
+Section Partial_order.
+
+ Context {X} {P: CPO X}.
+
+ #[global] Instance Equivalence_weq: Equivalence weq.
  Proof.
    constructor.
     intro x. now apply weq_spec.
     intros x y. rewrite 2weq_spec. tauto.
     intros x y z. rewrite 3weq_spec. split; transitivity y; tauto. 
-  Qed.
+ Qed.
+
  Global Instance PartialOrder_weq_leq: PartialOrder weq leq.
  Proof.
    intros x y. simpl. now rewrite weq_spec.
  Qed.
+ 
  Lemma antisym x y: x <= y -> y <= x -> x == y.
  Proof. rewrite weq_spec. tauto. Qed.
  
@@ -165,15 +124,14 @@ Qed.
  Lemma from_below x y: (forall z, z<=x <-> z<=y) -> x==y.
  Proof. intro E. apply antisym; apply E; reflexivity. Qed.
 
-(*
- Global Instance sup_leq:
-   Proper (leq ==> leq) sup.
- Proof.
-   intros P P' HP. apply sup_spec.
-   setoid_rewrite HP. 
-   now apply sup_spec.
- Qed.
- Global Instance sup_weq: Proper (weq ==> weq) sup := op_leq_weq_1.*)
+End Partial_order.
+
+
+(** * General properties of the sup operation. *)
+
+Section sup.
+
+ Context {X} {P: CPO X} `{L : CompleteLattice X}.
  
  Lemma leq_xsup D y: (Dbody D) y -> y <= sup D.
  Proof. intro H. now apply (sup_spec D). Qed.
@@ -181,86 +139,28 @@ Qed.
  Lemma leq_xsup_lat (Y:X->Prop) y : Y y -> y <= sup_lat Y.
  Proof. intro H. now apply (sup_spec_lat Y). Qed.
 
-Lemma sup_is_independent_of_proof : forall D_dir D_dir2, iff_part (Dbody D_dir) (Dbody D_dir2)
-  -> sup D_dir == sup D_dir2.
-Proof. 
+ Lemma sup_is_independent_of_proof : forall D_dir D_dir2, iff_part (Dbody D_dir) (Dbody D_dir2)
+   -> sup D_dir == sup D_dir2.
+ Proof. 
   intros. apply weq_spec. split; apply sup_spec; intros; apply leq_xsup;
   now apply H.
-Qed.
+ Qed.
 
-(*
-Lemma sup_unicity D s1 s2: sup D s1 -> sup D s2 -> s1 == s2.
-Proof.
-  intros. apply weq_spec. split; [apply (sup_spec D s1) | apply (sup_spec D s2)]; try assumption.
-  now apply (sup_spec D s2). now apply (sup_spec D s1).
-Qed.*)
-
-Program Definition empty {Y} {Q : CPO Y}: (directed_set leq) := exist _ (fun _ => False) _.
-Next Obligation.
-unfold Directed. (* unfold Directed_generalized.*) intros. contradict H.
-Defined.
-
-(* Above is better and equivalent, I keep this here to remember what I learned on Sig today *)
-(*
-Lemma empty_is_directed : (Directed (fun _ => False)).
-Proof. unfold Directed. intros. contradict H. Qed.
-Definition empty : directed_set := exist Directed (fun _ => False) empty_is_directed.
-*)
+ Program Definition empty {Y} {Q : CPO Y}: (directed_set leq) := exist _ (fun _ => False) _.
+ Next Obligation. unfold Directed. intros. contradict H. Defined.
 
  Definition bot := sup empty. (*Warning : with our current definition of directed,
- bottom exists since empty set is directed. Later, we will want to change that to allow bottom to no exist*)
+ bottom exists since the empty set is directed. Later, we might want to change that to allow bottom to no exist*)
+ 
  Lemma bot_spec: forall x, bot <= x.
  Proof. intro. now apply sup_spec. Qed.
 
- Definition top := sup_lat (fun _ => True).
- Lemma top_spec_lat: forall x, x <= top.
+ Definition top_lat := sup_lat (fun _ => True). (* Rmk : only exists in lattices, not just CPOs. *)
+ 
+ Lemma top_spec_lat: forall x, x <= top_lat.
  Proof. intro. now apply leq_xsup_lat. Qed.
-(*Not in CPOs ! We don't want CPOs to have a top, otherwise just word with Complete Lattices already.*)
 
-(* Following section : not really handy for CPOs, since cup and cap only exists if {x,y} is directed, 
-i.e. x and y are comparable. Forget it for now, may be of use later with lattices *)
-(*
- Definition cup x y := sup (fun z => z=x \/ z=y).
- Lemma cup_spec: forall x y z, Directed (fun z => z=x \/ z=y) -> cup x y <= z <-> (x <= z /\ y <= z).
- Proof.
-   intros. unfold cup. rewrite sup_spec.
-   now firstorder subst. apply H.
- Qed. (*small modif : need directedness in specification*)
-  Lemma cup_spec_lat: forall x y z, cup x y <= z <-> (x <= z /\ y <= z).
- Proof.
-   intros. unfold cup. rewrite sup_spec_lat.
-   now firstorder subst.
- Qed.
-
- Definition cap x y := sup (fun z => z<=x /\ z<=y).
- Lemma cap_spec: forall x y z, Directed (fun z => z<=x /\ z<=y) -> z <= cap x y <-> (z <= x /\ z <= y).
- Proof.
-   intros w y z D. unfold cap. split.
-   now intro H; split; rewrite H; apply sup_spec.
-   intros. now apply leq_xsup. 
- Qed. (*dunno if this will still be useful*)
- Lemma cap_spec_lat: forall x y z, z <= cap x y <-> (z <= x /\ z <= y).
- Proof.
-   intros. unfold cap. split.
-   now intro H; split; rewrite H; apply sup_spec_lat.
-   intros. now apply leq_xsup_lat. 
- Qed.
-*)
-
-
-(* --------------- Inf ---------------- *)
-
-(* Now defining an inf is also a problem... Usually we write it as the sup of elements lower than the set,
-but now there is no guarantee an inf exists (even if a sup exists btw).
-Two solutions : 
-1) Define the inf directly in the CPO with "downward" directed sets
-2) Define a "converse" CPO with reversed <= and define it as sup for this CPO.
---> Then we can make a lemma stating that the inf is actually the sup of lower elements 
-if this set is downward directed. 
-Try solution 2) to not "uselessly" weight down the definition of CPO.*)
-(* --> actually, no need for an inf ! We will instead define properties stating that an element is a least
-elements or things like that for the proofs. *)
-
+ (** Inf *)
 
  Definition inf_lat Y := sup_lat (fun z => forall y, Y y -> z <= y).
  Lemma inf_spec_lat: forall Y z, z <= inf_lat Y <-> (forall y, Y y -> z <= y).
@@ -272,156 +172,60 @@ elements or things like that for the proofs. *)
  
   Lemma leq_xinf (D: X -> Prop) y:  D y -> inf_lat D <= y.
  Proof. intro H. now apply inf_spec_lat with D. Qed.
- 
- (** other properties of binary joins *)
- (* Still cups, still not handy now*)
- (*
- Lemma leq_xcup x y z: Directed (fun t => t=x \/ t=y) -> z <= x \/ z <= y -> z <= cup x y.
+
+
+(* --- Inclusion of sets and sup --- *)
+
+ Definition included_body (S T : directed_set leq) := (Dbody S) ⊆ (Dbody T).
+ #[global] Instance sup_preserves_inclusion: Proper (included_body ==> leq) sup.
  Proof.
-  intro D. Check cup_spec.
-   destruct (cup_spec (cup x y) D).
-   intros [E|E]; rewrite E; now apply H.
- Qed.
-  Lemma leq_xcup_lat x y z: z <= x \/ z <= y -> z <= cup x y.
- Proof.
-   destruct (cup_spec_lat x y (cup x y)) as [H _].
-   now intros [E|E]; rewrite E; apply H.
+  intros S T HST. apply sup_spec. intros. apply leq_xsup.
+  now apply HST.
  Qed.
  
- Lemma cup_l x y: Directed (fun t => t=x \/ t=y) -> x <= cup x y.
- Proof. auto using leq_xcup. Qed.
-  Lemma cup_l_lat x y: x <= cup x y.
- Proof. auto using leq_xcup_lat. Qed.
- Lemma cup_r x y: Directed (fun t => t=x \/ t=y) -> y <= cup x y.
- Proof. auto using leq_xcup. Qed.
-  Lemma cup_r_lat x y: y <= cup x y.
- Proof. auto using leq_xcup_lat. Qed.
-*)
-
-(*Below is possible but not practical to write with directedness condition, 
-do it later if needed*)
-(*
- Lemma cupA_lat x y z: cup x (cup y z) == cup (cup x y) z.
- Proof.
-   apply from_above.
-   intro. rewrite !cup_spec_lat. tauto.
+ Definition iff_part_body (S T : directed_set leq) := iff_part (Dbody S) (Dbody T).
+ #[global] Instance sup_preserves_equality: Proper (iff_part_body ==> weq) sup.
+ Proof. 
+  intros S T HST. apply weq_spec. split; apply sup_preserves_inclusion; intros x Hx; now apply HST.
  Qed.
-
- Lemma cupC x y: Directed (fun t => t=x \/ t=y) -> cup x y == cup y x.
- Proof.
-   intro D.
-   apply from_above.
-   intro. rewrite !cup_spec. tauto.
-   rewrite directed_symmetry. apply D. now setoid_rewrite or_comm at 1.
-   apply D.
- Qed.
-  Lemma cupC_lat x y: cup x y == cup y x.
- Proof.
-   apply from_above.
-   intro. rewrite !cup_spec_lat. tauto.
- Qed.
-
-
- Lemma or_reduce : forall A, A \/ A <-> A.
- Proof. tauto. Qed.
- Lemma cupI x: cup x x == x. (*done more generally with CPOs*)
- Proof.
-   apply from_above.
-   intro. rewrite !cup_spec. tauto.
-   apply directed_symmetry with (fun z => z=x). (*intuition.*) now setoid_rewrite or_reduce.
-   apply singleton_is_directed.
- Qed.
-*)
-
-(* --- Inclusion of sets and includion of sups --- *)
-
-Definition included (S T: X -> Prop) := forall x, S x -> T x.
-Infix "⊆" := included (at level 70).
-
-#[global] Instance Included_trans : Transitive included.
-Proof.
-  intros Y1 Y2 Y3 H12 H13. intros x H. apply H13. now apply H12.
-Qed.
-
-Lemma sup_preserves_inclusion S T : (Dbody S) ⊆ (Dbody T) -> sup S <= sup T.
-Proof.
-  intro H. apply sup_spec. intros. apply leq_xsup.
-  now apply H.
-Qed.
-
-Lemma sup_preserves_eq S T : (forall x, (Dbody S) x <-> (Dbody T) x) -> sup S == sup T.
-Proof.
-  intros. apply weq_spec. split; apply sup_preserves_inclusion; 
-  [intros x Hx | intros x Hx]; now apply H.
-Qed.
-
-(*
-Lemma included_inf_is_greater S T : S ⊆ T 
-  -> Directed (fun z : X => forall y : X, S y -> z <= y)
- -> Directed (fun z : X => forall y0 : X, T y0 -> z <= y0) 
- -> inf T <= inf S.
-Proof.
-  intros H Ds Dt. apply inf_spec. assumption. intros. apply leq_xinf. assumption.
-  now apply H.
-Qed.
-Lemma inf_preserves_eq (S T : X -> Prop) : Directed (fun z : X => forall y : X, S y -> z <= y)
- -> Directed (fun z : X => forall y0 : X, T y0 -> z <= y0) -> (forall x, S x <-> T x) -> inf S == inf T.
-Proof.
-  intros. apply weq_spec. split; apply included_inf_is_greater; 
-  [intros x Hx | assumption | assumption | intros x Hx | assumption | assumption]; now apply H1.
-Qed.*)
 
 End sup.
-Global Hint Resolve bot_spec: core.
-(*Global Hint Resolve cup_l cup_r: core.*)
 
+Global Hint Resolve bot_spec: core.
+
+
+
+(** * Monotonous functions and other properties *)
 
 Section functions.
  Context {X} {P: CPO X}.
  
+ Definition Fix F x := F x == x.
+ Definition Post F x := x <= F x.
+ Definition Pre F x := F x <= x.
+ 
+ Lemma fix_is_post F : forall x, Fix F x -> Post F x.
+ Proof. intros. apply weq_spec in H. apply H. Qed.
+ Lemma fix_is_pre F : forall x, Fix F x -> Pre F x.
+ Proof. intros. apply weq_spec in H. apply H. Qed.
+ 
+ 
+ (* Monotonous functions *)
+ 
  Record mon := { body:> X -> X; Hbody: Proper (leq ==> leq) body }.
  
  #[global] Instance Hbody' (F:mon) : Proper (weq ==> weq) F.
- Proof.
-  apply (op_leq_weq_1 (Hf:=(Hbody F))).
-Qed.
+ Proof. apply (op_leq_weq_1 (Hf:=(Hbody F))). Qed.
 
-
-Inductive Image f (S : X -> Prop) : X -> Prop :=
+ Inductive Image f (S : X -> Prop) : X -> Prop :=
   |from_image : forall x, S x -> Image f S (f x).
 
-Definition Image' f (S : set X) (y:X) := exists x, S x /\ y = f x.
+ Definition Continuous f := forall (D : set X) (H : Directed leq D), {dir_im : Directed leq (Image f D) & 
+  f (sup (exist _ D H )) == sup (exist _ (Image f D) dir_im)}.
 
-Lemma im_eq : forall f S, iff_part (Image f S) (Image' f S).
-Proof.
-  intros f S x. split.
-  + intro. inversion H. now exists x0.
-  + intro. inversion H. destruct H0. rewrite H1. now apply from_image.
-Qed.
-
-Definition Continuous f := forall (D : set X) (H : Directed leq D), {dir_im : Directed leq (Image f D) & 
-  f (sup (exist _ D H )) == sup (exist _ (Image f D) dir_im)}. (*yup, dependent pair...*)
-
-(* Attempts at not making a dependent pair. Spoiler : it failed.*)
-(*
-Definition Continuous_im φ := forall (D: set X) (H:Directed leq D), Directed leq (Image φ D).
-
-Definition Continuous_1 φ := forall (D: set X) (H: Directed leq D), Directed leq (Image φ D).
-Definition Continuous φ := forall (D: set X) (H: Directed leq D), φ (sup (exist _ D H)) = sup (exist _ (Image φ D) (Continuous_1 φ D H)).
-
-Definition Image_dir φ S : (directed_set leq ):= exist _ (fun y => (exists x, y = φ x /\ ((Dbody S) x))) (Continuous_im φ).
-|from_image_dir : Continuous_im φ -> forall x, S x -> Image_dir φ S (φ x).
-
-Definition Continuous φ := forall (D: set X) (H:Directed leq D), Continuous_im φ /\ 
-  φ (sup (exist _ D H)) = sup (exist _ (Image φ D) (Continuous_im φ D H)).
-Next Obligation.
-  
-   /\ forall (D_dir:directed_set leq), φ (sup D_dir) = sup (exist (Directed leq) (Image φ (Dbody D_dir)) _).
-*)
-
-Lemma mon_preserves_directedness_and_sup (F:mon) : forall (D : set X) (H : Directed leq D), {dir_im : Directed leq (Image F D) & 
+ Lemma mon_preserves_directedness_and_sup (F:mon) : forall (D : set X) (H : Directed leq D), {dir_im : Directed leq (Image F D) & 
   sup (exist _ (Image F D) dir_im) <= F (sup (exist _ D H ))}.
-Proof.
+ Proof.
   intros. assert (Directed leq (Image F D)). 
   + unfold Directed. intros. inversion H0. inversion H1.
     destruct (H x0 x1); try assumption. exists (F x2).
@@ -429,509 +233,212 @@ Proof.
   + exists H0. apply sup_spec; cbn. intros.
     inversion H1. apply Hbody. now apply leq_xsup.
  Qed.
-
-(*same but with Image' to compare which definition is best in the proofs. And it seems to be less practical.*)
-Lemma mon_preserves_directedness_and_sup' (F:mon) : forall (D : set X) (H : Directed leq D), {dir_im : Directed leq (Image' F D) & 
-  sup (exist _ (Image' F D) dir_im) <= F (sup (exist _ D H ))}.
-Proof.
-  intros. assert (Directed leq (Image' F D)). 
-  + unfold Directed. intros. inversion H0. inversion H1.
-    destruct (H x0 x1); intuition. exists (F x2).
-    repeat split. now exists x2. rewrite H6. now apply Hbody.
-    rewrite H7. now apply Hbody.
-  + exists H0. apply sup_spec; cbn. intros.
-    inversion H1. destruct H2. rewrite H3. apply Hbody. now apply leq_xsup.
- Qed.
  
-
-End functions.
-
-
-
-
-
-(* Knaster-Tarski Theorem on Lattices *)
-
-Section lattice_results.
-Context {X} `{L: CompleteLattice X}.
- Variable b: mon.
-
- Definition gfp := sup_lat (fun x => x <= b x).
- Definition lfp := inf_lat (fun x => b x <= x).
-
- Proposition leq_gfp: forall y, y <= b y -> y <= gfp.
- Proof. apply leq_xsup_lat. Qed.
- Proposition geq_lfp: forall y, b y <= y -> lfp <= y.
- Proof. apply leq_xinf. Qed.
-
- Lemma gfp_pfp: gfp <= b gfp.
-Proof.
-  unfold gfp. apply sup_spec_lat. intros y H. rewrite H. apply Hbody.
-  apply leq_xsup_lat. apply H.
-Qed.
-Lemma lfp_pfp: b lfp <= lfp.
-Proof.
-  unfold lfp. apply inf_spec_lat. intros y H. rewrite <- H. apply Hbody.
-  apply leq_xinf. apply H.
-Qed.
-
- Lemma gfp_fp: gfp == b gfp.
-Proof.
-  rewrite weq_spec. split.
-    + apply gfp_pfp.
-    + apply leq_xsup_lat. apply Hbody. apply gfp_pfp.
-Qed.
-Lemma lfp_fp: lfp == b lfp.
-Proof.
-  rewrite weq_spec. split.
-    + apply leq_xinf. apply Hbody. apply lfp_pfp.
-    + apply lfp_pfp.
-Qed.
-End lattice_results.
-
-
-
-
-
-Section fixpoint.
- Context {X} {P: CPO X}.
-
- Definition Fix {Y} {Q : CPO Y} F x := F x == x.
- Definition Post {Y} {Q : CPO Y} F x := x <= F x.
- Definition Pre {Y} {Q : CPO Y} F x := F x <= x.
  
- Lemma fix_is_post F : forall x, Fix F x -> Post F x.
- Proof. intros. apply weq_spec in H. apply H. Qed.
- Lemma fix_is_pre F : forall x, Fix F x -> Pre F x.
- Proof. intros. apply weq_spec in H. apply H. Qed.
+ (* Some basic monotonous functions *)
  
- (* Obsolete : we can't really define mu, it doesn't even always exists.
- However, we can define a property stating that we are the least element of a set*)
-
-Definition is_least {Y} {Q : CPO Y} S x := S x /\ forall y, S y -> x <= y.
-Definition is_inf {Y} {Q : CPO Y} S x := forall z, (forall y, S y -> z <= y) <-> z <= x.
-Definition is_greatest {Y} {Q : CPO Y} S x := S x /\ forall y, S y -> y <= x.
-Definition is_sup {Y} {Q : CPO Y} S x := forall z, (forall y, S y -> y <= z) <-> x <= z.
-
-Lemma test_coherence1 : forall D, is_sup (Dbody D) (sup D).
-Proof. intros D z. split; apply sup_spec. Qed.
-Lemma test_coherence2 : forall D, (Dbody D) (sup D) -> is_greatest (Dbody D) (sup D).
-Proof. intros. split. assumption. now apply sup_spec. Qed.
+ Program Definition const x: mon := {| body y := x |}.
+ Next Obligation. intros ? ? ?. reflexivity. Qed.
  
- (*
- Notation µ F := (inf (fun x => Fix F x)). (*Rmq : Attention, on préférerait que ce soit un min.
- Cependant, s'il existe, il est égal à l'inf donc c'est bon.*)
+ Definition id: mon := {| 
+   body x := x; 
+   Hbody x y H := H 
+ |}.
  
- Definition mu_exists F := Directed (fun z => forall y, (fun x => Fix F x) y -> z <= y) /\ Fix F (µ F).
- *)
+ Definition comp {Y} {Q : CPO Y} (f g: mon): mon := {|
+   body := fun x => f (g x); 
+   Hbody x y H := Hbody f _ _ (Hbody g _ _ H) 
+ |}.
+ Infix "°" := comp (at level 20): CPO. 
+ 
+ 
+ (* Iterations of a function *)
  
  Fixpoint itere F n x0 : X := match n with
   | 0 => x0
   | S m => F (itere F m x0)
- end.
+ end. (*Indexed by n for simplicity on comparison properties.*)
 
-Lemma itere_monotony (F:mon) : forall n, Proper (leq ==> leq) (itere F n).
-Proof.
-  intros n x y H. induction n. now cbn. cbn. now apply Hbody.
-Qed.
+ Lemma itere_monotony (F:mon) : forall n, Proper (leq ==> leq) (itere F n).
+ Proof. intros n x y H. induction n. now cbn. cbn. now apply Hbody. Qed.
 
-(*
- Inductive iteres F : X -> Prop :=
-  | iteres_0 : (iteres F bot)
-  | iteres_S : forall x, (iteres F x) -> (iteres F (F x)).
-*)
+ Lemma chain_itere (F:mon) : forall (n : nat), itere F n bot <= itere F (S n) bot.
+ Proof. intro n. induction n. now cbn. cbn. now apply Hbody. Qed.
 
-Lemma chain_itere (F:mon) : forall (n : nat), itere F n bot <= itere F (S n) bot.
-Proof.
-  intro n. induction n. now cbn.
-  cbn. now apply Hbody.
-Qed.
-
-Lemma chain_increase (F:mon) : forall (m n : nat), le n m -> itere F n bot <= itere F m bot.
-Proof.
+ Lemma chain_increase (F:mon) : forall (m n : nat), le n m -> itere F n bot <= itere F m bot.
+ Proof.
   intros m n H. induction m. now inversion H.
   inversion H. easy.
   rewrite <- chain_itere. now apply IHm.
-Qed.
+ Qed.
 
-Lemma itere_preserves_fix (F:mon) : forall β n, Fix F β -> (itere F n β) == β.
-Proof.
+ Lemma itere_preserves_fix (F:mon) : forall β n, Fix F β -> (itere F n β) == β.
+ Proof.
   intros. induction n. now cbn. cbn. unfold Fix in H. rewrite <- H at 2.
   now apply Hbody'.
-Qed.
+ Qed.
 
-Inductive iteres F : X -> Prop := 
+ Inductive iteres F : X -> Prop := 
   | from_bot : forall n, iteres F (itere F n bot).
 
-
-(* This is already done by "inversion" on a <= *)
-(*
-Lemma inf_eq : forall (n m : nat), le n m -> n = m \/ le (S n) m.
-Proof. 
-  intros. inversion H. now left.
-  right. now apply le_n_S.
-Qed.
-*)
-
-(*3 lemmas below are actually useless, see le_ge_dec...
-(Plus they already exist in Arith...)*)
-Lemma compare_eq: forall e f, Nat.compare e f = Eq -> e=f.
-Proof.
-  induction e; destruct f; cbn; try discriminate.
-  - reflexivity.
-  - intro H. now rewrite IHe with f.
-Qed.
-
-Lemma compare_Lt: forall n m, Nat.compare n m = Lt -> n < m.
-Proof. 
-induction n; destruct m; cbn; try discriminate; intro H.
-  + lia.
-  + assert (n < m). now apply IHn. lia.
-Qed.
-
-Lemma compare_Gt: forall n m, Nat.compare n m = Gt -> m < n.
-Proof. 
-induction n; destruct m; cbn; try discriminate; intro H.
-  + lia.
-  + assert (m < n). now apply IHn. lia.
-Qed.
-
-(*
-Lemma comparison : forall (n m:nat), le n m \/ le m n.
-Proof. intros n m. case_eq
-*)
-
-Lemma iteres_directed (F:mon): Directed leq (iteres F).
-Proof.
+ Lemma iteres_directed (F:mon): Directed leq (iteres F).
+ Proof.
   unfold Directed. intros. destruct H. destruct H0.
-  case_eq (Nat.compare n n0); intro H.
-  + exists (itere F n bot). repeat split. easy. now rewrite compare_eq with n n0.
-  + exists (itere F n0 bot). repeat split. apply chain_increase. 
-  assert (n < n0). now apply compare_Lt. lia. reflexivity.
-  + exists (itere F n bot). repeat split. reflexivity.
-  apply chain_increase. assert (n0 < n). now apply compare_Gt. lia.
-  Restart. unfold Directed. intros. destruct H. destruct H0.
   destruct le_ge_dec with n n0.
   + exists (itere F n0 bot). repeat split. now apply chain_increase. reflexivity.
   + exists (itere F n bot). repeat split. reflexivity. now apply chain_increase.
-Qed.
-
-(*
-Program Definition iteres_dir (F:mon) := (exist _ (iteres F) (iteres_directed F)).*)
-(*Program Definition α (F:mon) := (sup (exist _ (iteres F) _)).
-Next Obligation. apply (iteres_directed F). Qed.*)
-(* Notation α F := (sup (iteres F)).*)
-Definition α (F:mon) := (sup (exist (Directed leq) (iteres F) (iteres_directed F))).
-
- Theorem Fixpoint_I_i (F:mon) : Fix F (α F) -> is_least (Fix F) (α F).
- Proof.
- intro H. split; try assumption.
-  intros. apply sup_spec; cbn. intros z Q.
-  inversion Q. rewrite <- (itere_preserves_fix F y n).
-  now apply itere_monotony. assumption.
-Qed.
-
-
-(* ---------------------- Theorem I (ii) ---------------------------------- *)
-
-Inductive iteres_from_1 F : X -> Prop := 
+ Qed.
+ 
+ Inductive iteres_from_1 F : X -> Prop := 
   | from_bot_from_1 : forall n,  le 1 n -> iteres_from_1 F (itere F n bot).
   
-Lemma iteres_from_1_directed (F:mon): Directed leq (iteres_from_1 F).
-Proof.
+ Lemma iteres_from_1_directed (F:mon): Directed leq (iteres_from_1 F).
+ Proof.
   unfold Directed. intros. destruct H. destruct H0.
   destruct le_ge_dec with n n0.
   + exists (itere F n0 bot). repeat split. assumption. now apply chain_increase. reflexivity.
   + exists (itere F n bot). repeat split. assumption. reflexivity. now apply chain_increase.
-Qed.
+ Qed.
 
-Lemma image_of_iteres F : forall x, (Image F (iteres F)) x <-> (iteres_from_1 F) x.
-Proof. (*TODO : rewrite this with iff_part ? And add a reserved notation for iff_part.*)
+ Lemma image_of_iteres F : iff_part (Image F (iteres F)) (iteres_from_1 F).
+ Proof.
   intro. split; intro; inversion H. inversion H0.
   + assert (iteres_from_1 F (itere F (S n) bot)). apply from_bot_from_1. lia.
     apply H3.
   + induction n. contradict H0. lia.
     cbn. apply from_image. apply from_bot.
-Qed.
+ Qed.
 
-Lemma from_1_included F : included (iteres_from_1 F) (iteres F).
-Proof.
-  intros x H. inversion H. apply from_bot.
-Qed.
+ Lemma from_1_included F : included (iteres_from_1 F) (iteres F).
+ Proof. intros x H. inversion H. apply from_bot. Qed.
 
-Program Definition α' (F:mon) := (sup (exist _ (iteres_from_1 F) _)).
-Next Obligation. apply iteres_from_1_directed. Qed.
-
-Lemma sup_from_1 (F:mon) : α F == α' F.
-Proof.
-  apply weq_spec. split. 
-  + apply sup_spec; cbn. intros. inversion H.
-  induction n. now cbn. apply leq_xsup.
-  apply from_bot_from_1. lia.
-  + apply sup_preserves_inclusion; cbn. apply from_1_included.
-Qed.
-
-(* Fix F (mu F) is here to say that "mu F exists", cause it is supposed to be a min and not an inf. *)
-Theorem Fixpoint_I_ii (F:mon) : Continuous F -> is_least (Fix F) (α F).
-Proof.
-  intro H.
-  assert (Fix F (α F)).
-   + unfold Fix. destruct (H (iteres F) (iteres_directed F)) as [HD HS].
-    transitivity (α' F); try now rewrite sup_from_1. rewrite HS.
-    apply sup_is_independent_of_proof. cbn. unfold iff_part. apply image_of_iteres.
-   + now apply Fixpoint_I_i.
-Qed.
+End functions.
 
 
+Section Particular_CPOs.
 
-(* ------------------------- Theorem II ------------------------------ *)
+ Context {X} {P: CPO X}.
 
-(*
-Notation µ0 F := (inf (fun x => Pre F x)). 
- Definition mu0_exists F := Directed (fun z => forall y, (fun x => Pre F x) y -> z <= y) /\ Pre F (µ0 F).*)
-(*Warning : this is delicate. "If the least prefixpoint exists, we write it mu0" is not easily written in Coq.
-I could also replace mu0_exists (and mu_exists) with the properties of a least prefixpoint, but to prove it from
-the def of the inf I would still need the inf to be well defined, ie. this set to be directed.
-I think it could be possible for this set to NOT be directed (so inf not well defined), but for such a least prefixpoint
-to still exist. In that case I will not know how to define it at all. It will just be a "exists" proposition.*)
-
-(* --> is_least (Pre F) x already means what I want.*)
-
-Lemma Induction_Rule (F:mon) : (exists µ0, is_least (Pre F) µ0)
-  -> exists µ, is_least (Fix F) µ /\ forall x, Pre F x -> µ <= x.
-Proof.
-  intro H. destruct H as [µ0 Hmu0].
-  exists µ0. repeat split.
-  + apply weq_spec. split. apply Hmu0.
-    apply Hmu0. unfold Pre. apply Hbody. apply Hmu0.
-  + intros. apply Hmu0. now apply fix_is_pre.
-  + apply Hmu0.
-Qed.
-
-
-
-(* Lemma 8.21*)
-
-Program Definition const x: mon := {| body y := x |}.
- Next Obligation. intros ? ? ?. reflexivity. Qed.
-
- (** identity and composition
-     the monotonicity proofs are transparent to get strong equalities
-     - [id ° f = f ° id = f], and
-     - [f ° (g ° h) = (f ° g) ° h]
-  *)
- Definition id {Y} {Q : CPO Y}: mon := {| 
-   body x := x; 
-   Hbody x y H := H 
- |}.
-
- Definition comp {Y} {Q : CPO Y} (f g: mon): mon := {|
-   body := fun x => f (g x); 
-   Hbody x y H := Hbody f _ _ (Hbody g _ _ H) 
- |}.
- Infix "°" := comp (at level 20): CPO.
- 
-
-
-Program Instance CPO_mon {Y} {Q : CPO Y}: CPO mon := {|
-   weq := pointwise_relation Y weq;
-   leq := pointwise_relation Y leq;
+ Program Instance CPO_mon : CPO mon := {|
+   weq := pointwise_relation X weq;
+   leq := pointwise_relation X leq;
    sup F := {| body a := sup (fun b => exists2 f, F f & b=f a) |};
  |}.
-Next Obligation.
+ Next Obligation.
   unfold Directed. intros. destruct F as [SF D]; cbn in *.
   destruct H as [fx Hfx]. destruct H0 as [fy Hfy].
   destruct (D fx fy) as [f [Hf1S [Hff1 Hff2]]]; try assumption.
   exists (f a). repeat split. now exists f.
   + rewrite H. apply Hff1.
   + rewrite H0. apply Hff2.
-Qed.
-Next Obligation.
+ Qed.
+ Next Obligation.
   destruct F as [SF D]; cbn in *.
   intros x y H. apply sup_spec; cbn. intros.
   destruct H0 as [f Hf].
   transitivity (f y). rewrite H0. now apply Hbody.
   apply leq_xsup. cbn. now exists f.
-Qed.
-Next Obligation. (*Rmk : symbol ":>" is to declare a trivial instance.*)
+ Qed.
+ Next Obligation. (*Rmk : symbol ":>" is to declare a trivial instance.*)
   apply Build_PreOrder.
   + intro x. reflexivity.
   + intros f g h Hfg Hgh x. now transitivity (g x).
-Qed.
-Next Obligation.
+ Qed.
+ Next Obligation.
   split; intros.
   + split; intro a; now apply weq_spec.
   + intro. now apply weq_spec.
-Qed.
-Next Obligation.
+ Qed.
+ Next Obligation.
   destruct D as [SF D]; cbn in *. split. 
   + intros H f Df x. rewrite <- (H x).
   eapply sup_spec. reflexivity. cbn. now exists f.
   + intros H x. apply sup_spec. intros. inversion H0. rewrite H2. now apply (H x0).
-Qed.
+ Qed.
 
-Program Instance CPO_parts: CPO (set X) := {|
+ Program Instance CPO_parts: CPO (set X) := {|
    weq := iff_part;
    leq := included;
    sup A := (fun x => exists Y, A Y /\ Y x);
  |}.
-Next Obligation.
+ Next Obligation.
   apply Build_PreOrder.
   + intro Y. now intro x.
   + apply Included_trans.
-Qed.
-Next Obligation.
+ Qed.
+ Next Obligation.
   repeat split; try intuition; intros a; intro H0; apply H; try apply H0.
-Qed.
-Next Obligation.
+ Qed.
+ Next Obligation.
   split; intros; intros a Ha. apply H. now exists y.
   destruct Ha. apply (H x). apply H0. apply H0.
-Qed.
+ Qed.
 
-Program Instance Lattice_parts : CompleteLattice (CPO_parts) := {|
+ Program Instance Lattice_parts : CompleteLattice (CPO_parts) := {|
   sup_lat A := (fun x => exists Y, A Y /\ Y x); 
  |}.
-Next Obligation.
+ Next Obligation.
   split; intros; intros a Ha. apply H. now exists y.
   destruct Ha. apply (H x). apply H0. apply H0.
-Qed.
+ Qed.
 
-Definition Increasing {Y} {Q : CPO Y} (*(F: @mon Y Q)*) (G : Y -> Y) := forall (x:Y), x <= G x.
-Check Increasing.
 
-(*Note : from now on, have to detail the type used for mon, since last instance declared is used to infer type,
-here it is now mon on the CPO of mon.*)
+ (** * sub-CPO : Define a set (part of X) as being a CPO *)
 
-(*
-Set Printing Implicit.
+ Definition is_subCPO (Y : set X) := forall D, included (Dbody D) Y -> Y (sup D).
 
-(* Class indexed by a type *)
-Class foo {X : Type} := {bar : X -> X }.
+ Definition down (x:X) := (fun z => z <= x).
 
-(* Two instances for the class *)
-Context {foo1 : @foo nat}.
-Context {foo2 : @foo (nat -> nat)}.
+ Lemma down_is_subCPO : forall x, is_subCPO (down x).
+ Proof. intros x D Hd. unfold down. apply sup_spec. intros. now apply Hd. Qed.
 
-(* A function indexed by an instance of [foo] *)
-Variable (f : forall {X} {F: @foo X}, Type).
+ Definition set_type (Y : set X) : Type := { x : X | Y x}.
+ Definition element Y (y :set_type Y) := proj1_sig y.
 
-(* The last instance defined has priority: `f`
-   gets implicitly typed at [foo (nat -> nat)] *)
-Definition testf := f.
-Definition testf2 := @f nat _.
+ Definition complete_body {Y : set X} (D : set (set_type Y)) : set X := 
+  (fun x => {is_in_Y : Y x & D (exist _ x is_in_Y)}).
 
-(* So naturally the identity over unspecified [f] gets inferred
-   as the identity over [f (nat -> nat)] *)
-Definition test2 (b : f) : f  := b.
-(* But somehow more surprising: the instances of both the argument and the return type are inferred completely independently: explicitly specifying one of the two leads in a type error as the first argument still got typed at [f (nat -> nat)] *)
-Fail Definition test3 (b : f) : @f nat _  := b.
-Fail Definition test3 (b : @f nat _) : f  := b.
-Definition test3 (b : @f nat _) : @f nat _  := b.
-*)
+ Program Definition subCPO (*{X} {P : CPO X}*) (Y:set X) (H : is_subCPO Y) : (CPO (set_type Y)) := {|
+   weq x y := (@weq X P) (element x) (element y);
+   leq x y := (@leq X P) (element x) (element y);
+   sup D := (@sup X P) (exist (Directed leq) (complete_body (Dbody D)) _) ;
+ |}.
+ Next Obligation. 
+  destruct D as [D Hd]. cbn. intros x y Hx Hy. inversion Hx. inversion Hy.
+  destruct (Hd (exist (fun x : X => Y x) x x0) (exist (fun x : X => Y x) y x1)) 
+    as [[z Pz] [Hz [Hxz Hyz]]]; try assumption.
+  exists z. split. now exists Pz. now split.
+ Qed.
+ Next Obligation.
+  apply H. intros x Hx.
+  destruct D as [D Hd]; cbn in Hx. now destruct Hx.
+ Qed.
+ Next Obligation. apply Build_PreOrder; intro x. reflexivity. intros y z Hxy Hyz. now transitivity (element y). Qed.
+ Next Obligation. apply weq_spec. Qed.
+ Next Obligation. split.
+  + intros. apply (sup_spec (exist (Directed leq) (complete_body (Dbody D)) (subCPO_obligation_1 D))); cbn.
+    assumption. destruct y. cbn. now exists y.
+  + intros. apply sup_spec. cbn. intros. destruct H1. now apply (H0 (exist (fun x : X => Y x) y x)).
+ Qed.
 
-(*Program Definition I := exist _ Increasing _.*)
 
-Program Definition I {Y} {Q : CPO Y} := exist (Directed (@leq mon CPO_mon)) (Increasing (*:set (@mon X P)*)) _. 
-Next Obligation.
-  (*unfold I_obligation_1.*)
-  unfold Directed. intros f g Hf Hg. exists (comp f g). repeat split.
-  + intro x. transitivity (g x). apply Hg. apply Hf.
-  + intro x. cbn. apply Hbody. apply Hg.
-  + intro x. cbn. apply Hf.
-Defined.
+(* Some instances that can now be defined on CPO_parts and CPO_mon. *)
 
-Definition H_sup {Y} {Q : CPO Y} := (sup I).
+ Variable F : X -> X.
 
-Lemma H_sup_is_increasing {Y} {Q : CPO Y} : Increasing H_sup.
-Proof. intro. assert (id <= H_sup). now apply (sup_spec I). apply H. Qed.
+ #[global] Instance image_eq : Proper (weq ==> weq) (Image F).
+ Proof. intros Y1 Y2 HY. split; intro H; inversion H; apply from_image; now apply HY. Qed.
 
-(*Variante constructive :*)
-Lemma H_sup_bot_is_fix_point_of_all_Increasing {Y} {Q : CPO Y} (F:@mon Y Q) : 
-  Increasing F -> Fix F (H_sup bot).
-Proof.
-  intro. assert ((comp F H_sup) == H_sup).
-  + apply weq_spec. split. apply (sup_spec I). reflexivity. 
-    intro x. transitivity (H_sup x). apply H_sup_is_increasing. apply H.
-    intro. apply H.
-  + unfold Fix. now setoid_rewrite (H0 bot).
-Qed.
+ #[global] Instance set_incl : Proper (weq ==> weq ==> iff) included.
+ Proof. intros Y1 Y2 H12 Y3 Y4 H34. split; intros Hi x Hx; apply H34; apply Hi; now apply H12. Qed.
 
-(*below : a simpler version of lemma 8.21 used in theorem. Only need existence of a FixPoint,
-not of a common Fixpoint for all Increasing function.*)
-Lemma increasing_has_fix_point {Y} {Q : CPO Y} (F:@mon Y Q) : Increasing F -> exists (x:Y), Fix F x.
-Proof.
-  intro. exists (H_sup bot). now apply H_sup_bot_is_fix_point_of_all_Increasing.
-Qed.
-
-Definition Invariant {Y} {Q : CPO Y} F (Y0: set Y) := included (Image F Y0) Y0.
-
-Definition is_subCPO {Y} {Q' : CPO Y} (Q:set Y) := forall D, included (Dbody D) Q -> Q (sup D).
-
-Variable F : (@mon X P).
-
-Definition P0 {Y} {Q : CPO Y} (F:Y->Y) := 
-  (fun x => forall Y, Invariant F Y -> is_subCPO Y -> Y x). 
-(* intersection of all invariant sub-CPOs *)
-
-Lemma P0_is_invariant_subCPO {Yt} {Q : CPO Yt} (F':Yt->Yt) : Invariant F' (P0 F') /\ is_subCPO (P0 F').
-Proof.
-  split.
-  + intros x H. inversion H. intros Y Hi Hs. apply Hi. apply from_image. now apply (H0 Y).
-  + intros D H Y Hi Hs. apply Hs. rewrite H. intros x Hx. now apply Hx.
-Qed.
-
-Lemma P0_is_smallest_invariant_subCPO {Yt} {Q : CPO Yt} (F':Yt->Yt) : forall Y, Invariant F' Y -> is_subCPO Y -> included (P0 F') Y.
-Proof. intros Y Hi Hs x Hx. now apply Hx. Qed.
-
-Program Definition Φ F' : @mon (set X) (CPO_parts) :=  (*since def of mon is linked to that of CPOs, need a CPO of parts*)
-  {| body X := (fun x => (x = bot \/ (Image F' X) x \/ (exists D, included (Dbody D) X /\ x = sup D))) |}.
-Next Obligation.
-  intros Y1 Y2 H12 x Hx. destruct Hx; intuition. 
-  + right. left. inversion H0. apply from_image. now apply H12.
-  + destruct H0 as [Hd [Hi Hs]]. right. right. exists Hd. split.
-    intros y Hy. apply H12. now apply Hi. assumption.
-Qed.
-
-Definition P0' F' := lfp (Φ F'). (* sup_lat (fun x => x <= Φ F x).*)
-Check P0.
-Check P0'.
-
-Instance image_eq : Proper (weq ==> weq) (Image F).
-Proof. intros Y1 Y2 HY. split; intro H; inversion H; apply from_image; now apply HY. Qed.
-(*Instance set_incl : Proper (weq ==> iff_part) included.
-Proof. intros Y1 Y2 HY Y3. split; intros Hi x Hx; apply Hi; now apply HY. Qed.*)
-
-Instance set_incl : Proper (weq ==> weq ==> iff) included.
-Proof. intros Y1 Y2 H12 Y3 Y4 H34. split; intros Hi x Hx; apply H34; apply Hi; now apply H12. Qed.
-
-(*Instance test (F:@mon X P) Y : Proper (weq ==> Basics.flip Basics.impl) (included Y).
-Proof. intros Y1 Y2 HY H x Hx. apply HY. now apply H. Qed.*)
-
-Lemma set_eq : forall (f g : set X), f == g -> (pointwise_relation X iff) f g.
-Proof.
+ Lemma set_eq : forall (f g : set X), f == g -> (pointwise_relation X iff) f g.
+ Proof.
   intros f g H x. split; intro Hh; apply weq_spec in H; destruct H.
   now apply H. now apply H0.
-Qed.
+ Qed.
 
-(*
-Definition appliance (A: Type) := fun (f:A->A) => fun x => f x. About eq. About appliance.
-
-Instance set_eq : Proper (weq ==> (pointwise_relation X iff)) appliance.
-Proof.
-  intros Y1 Y2 HY. split;
-*)
-(*
-Instance weq_sym : Symmetric weq.
-Admitted.
-
-Ltac rew H H' := eapply set_eq in H'; [| (exact H || (symmetry; exact H))].
-Tactic Notation "prew" hyp(H) "in" hyp(H') := rew H H'.
-*)
-
-
-
-
-
+End Particular_CPOs.
 
 
 Ltac rew H H' :=
@@ -951,65 +458,222 @@ Tactic Notation "prew" constr(H) "in" hyp(H') := rew H H'.
 Tactic Notation "prew" hyp(H)    := rew_goal H.
 Tactic Notation "prew" constr(H) := rew_goal H.
 
-(* Tests *)
-(*
-Variable (f g : X -> Prop).
-Axiom (EQ: f == g).
-
-Goal forall (x : X) (H : f x), False.
-  intros.
-  prew EQ in H.
-Abort.
-
-Goal forall (f g : X -> Prop) (x : X) (EQ' : f == g) (H : f x), False.
-  intros.
-  prew EQ' in H.
-Abort.
-
-Goal forall (x : X), f x.
-  intros.
-  prew EQ.
-Abort.
-
-Goal forall (f g : X -> Prop) (x : X) (EQ' : f == g), f x.
-  intros.
-  prew EQ'.
-Abort.
-*)
-
-(* Previous attempts :*)
-(*
-Ltac pointed_rewrite H H' := match type of H with | _ ?x => apply (set_eq H) in H' end.
-  Tactic Notation "prew" hyp(H) "in" hyp(H') := pointed_rewrite H H'.
-*)
 
 
-(*Tactic Notation prew Y1 'in' Y2 := pointed_rewrite Y1 Y2.*)
+(** * Common fixpoint of every monotonous increasing function *)
 
-(*
-Instance test f g: (respectful weq (pointwise_relation Prop iff)) f g.
+Section Increasing_fixpoint.
+ Context {X} {P: CPO X}.
+ 
+ Definition Increasing F := forall x, x <= F x.
 
-Instance obvious : Proper (weq ==> Basics.flip Basics.impl) (pointwise_relation iff).
-Lemma equal_sets_give_same_props : forall Y1 Y2, Y1 == Y2 -> forall x, Y1 x <-> Y2 x.
-Proof. intros. split.
-*)
+ Definition leq_mon := (@leq mon CPO_mon).
+ Definition weq_mon := (@weq mon CPO_mon).
+
+ Program Definition Increasing_functions := exist (Directed leq_mon) Increasing _. 
+ Next Obligation.
+  unfold Directed. intros f g Hf Hg. exists (comp f g). repeat split.
+  + intro x. transitivity (g x). apply Hg. apply Hf.
+  + intro x. cbn. apply Hbody. apply Hg.
+  + intro x. cbn. apply Hf.
+ Defined.
+
+ Definition H_sup := (sup Increasing_functions).
+
+ Lemma H_sup_is_increasing : Increasing H_sup.
+ Proof. intro. assert (leq_mon id H_sup). now apply (sup_spec Increasing_functions). apply H. Qed.
+
+ Lemma H_sup_bot_is_fixpoint_of_all_Increasing (F:mon) : 
+  Increasing F -> Fix F (H_sup bot).
+ Proof.
+  intro. assert (weq_mon (comp F H_sup) H_sup).
+  + apply weq_spec. split. apply (sup_spec Increasing_functions). reflexivity. 
+    intro x. transitivity (H_sup x). apply H_sup_is_increasing. apply H.
+    intro. apply H.
+  + unfold Fix. now setoid_rewrite (H0 bot).
+ Qed.
+
+ (* Lemma 8.21*)
+ Lemma increasing_has_fix_point (F:mon) : Increasing F -> exists x, Fix F x.
+ Proof.
+  intro. exists (H_sup bot). now apply H_sup_bot_is_fixpoint_of_all_Increasing.
+ Qed.
+
+ End Increasing_fixpoint.
 
 
-Lemma P0_is_P0' F' : (P0 F') == (P0' F').
-Proof.
+
+(** * Invariant subCPOs *)
+
+Section Invariant_subCPOs.
+ 
+ Context {X} {P: CPO X}.
+ 
+ Definition Invariant (F : X -> X) Y := included (Image F Y) Y.
+
+Variable F : X -> X.
+
+ Definition P0 :=  (*P0 is the smallest invariant subCPO : intersection of all invariant sub_CPOs.*)
+  (fun x => forall Y, Invariant F Y -> is_subCPO Y -> Y x).
+
+ Lemma P0_is_invariant_subCPO : Invariant F P0 /\ is_subCPO P0.
+ Proof.
+  split.
+  + intros x H. inversion H. intros Y Hi Hs. apply Hi. apply from_image. now apply (H0 Y).
+  + intros D H Y Hi Hs. apply Hs. rewrite H. intros x Hx. now apply Hx.
+ Qed.
+
+ Lemma P0_is_smallest_invariant_subCPO : forall Y, Invariant F Y -> is_subCPO Y -> included P0 Y.
+ Proof. intros Y Hi Hs x Hx. now apply Hx. Qed.
+
+End Invariant_subCPOs.
+
+
+
+(* Knaster-Tarski Theorem on Lattices *)
+
+Section lattice_results.
+ Context {X} `{L: CompleteLattice X}.
+ Variable b: mon.
+
+ Definition gfp := sup_lat (fun x => x <= b x).
+ Definition lfp := inf_lat (fun x => b x <= x).
+
+ Proposition leq_gfp: forall y, y <= b y -> y <= gfp.
+ Proof. apply leq_xsup_lat. Qed.
+ Proposition geq_lfp: forall y, b y <= y -> lfp <= y.
+ Proof. apply leq_xinf. Qed.
+
+ Lemma gfp_pfp: gfp <= b gfp.
+ Proof.
+  unfold gfp. apply sup_spec_lat. intros y H. rewrite H. apply Hbody.
+  apply leq_xsup_lat. apply H.
+ Qed.
+ Lemma lfp_pfp: b lfp <= lfp.
+ Proof.
+  unfold lfp. apply inf_spec_lat. intros y H. rewrite <- H. apply Hbody.
+  apply leq_xinf. apply H.
+ Qed.
+
+ Lemma gfp_fp: gfp == b gfp.
+ Proof.
+  rewrite weq_spec. split.
+    + apply gfp_pfp.
+    + apply leq_xsup_lat. apply Hbody. apply gfp_pfp.
+ Qed.
+ Lemma lfp_fp: lfp == b lfp.
+ Proof.
+  rewrite weq_spec. split.
+    + apply leq_xinf. apply Hbody. apply lfp_pfp.
+    + apply lfp_pfp.
+ Qed.
+
+End lattice_results.
+
+
+
+Section Using_Tarski.
+(* Remark : although this section is used in the proofs of the book, it is not used throughout this file.
+It is enough to work with P0 as the smallest invariant subCPO, no need to use its properties of least fixpoint. *)
+
+ Context {X} {P: CPO X}.
+
+ Program Definition Φ F' : @mon (set X) (CPO_parts) :=  (*since def of mon is linked to that of CPOs, need a CPO of parts*)
+  {| body X := (fun x => (x = bot \/ (Image F' X) x \/ (exists D, included (Dbody D) X /\ x = sup D))) |}.
+ Next Obligation.
+  intros Y1 Y2 H12 x Hx. destruct Hx; intuition. 
+  + right. left. inversion H0. apply from_image. now apply H12.
+  + destruct H0 as [Hd [Hi Hs]]. right. right. exists Hd. split.
+    intros y Hy. apply H12. now apply Hi. assumption.
+ Qed.
+
+ Definition P0' F' := (@lfp (set X) CPO_parts Lattice_parts) (Φ F').
+
+ Lemma P0_is_P0' F : (@weq (set X) CPO_parts) (P0 F) (P0' F).
+ Proof.
   apply weq_spec. split.
   + apply P0_is_smallest_invariant_subCPO.
     - unfold Invariant. unfold P0'. rewrite lfp_fp at 2.
       intros x H. right. now left.
     - unfold is_subCPO. unfold P0'. intros D H.
-      prew (lfp_fp (Φ F')). (*apply (set_eq (lfp_fp (Φ F))).*)
+      apply (set_eq (lfp_fp (Φ F))). (* prew does not work *)
       right. right. now exists D.
-  + unfold P0'. Print leq_gfp. apply geq_lfp. intros x H.
-    destruct (@P0_is_invariant_subCPO X P F'). destruct H. rewrite H.
+  + unfold P0'. apply geq_lfp. intros x H.
+    destruct (P0_is_invariant_subCPO F). destruct H. rewrite H.
     apply (H1 empty). intros y Hy. contradict Hy.
     destruct H. inversion H. apply H0. now apply from_image.
     destruct H as [D [Hd Hs]]. rewrite Hs. now apply (H1 D).
-Qed.
+ Qed.
+
+End Using_Tarski.
+
+
+
+(** * Fixpoint theorems ! *)
+
+Section Fixpoints.
+ Context {X} {P: CPO X}.
+
+ Definition is_least {Y} {Q : CPO Y} S x := S x /\ forall y, S y -> x <= y.
+ Definition is_inf {Y} {Q : CPO Y} S x := forall z, (forall y, S y -> z <= y) <-> z <= x.
+ Definition is_minimal {Y} {Q : CPO Y} S x := S x /\ forall y, S y -> y <= x -> y == x.
+ Definition is_greatest {Y} {Q : CPO Y} S x := S x /\ forall y, S y -> y <= x.
+ Definition is_sup {Y} {Q : CPO Y} S x := forall z, (forall y, S y -> y <= z) <-> x <= z.
+
+ Lemma test_coherence1 : forall D, is_sup (Dbody D) (sup D).
+ Proof. intros D z. split; apply sup_spec. Qed.
+ Lemma test_coherence2 : forall D, (Dbody D) (sup D) -> is_greatest (Dbody D) (sup D).
+ Proof. intros. split. assumption. now apply sup_spec. Qed.
+
+
+ (** * Fixpoint theorems and proofs : first theorem. *)
+ Variable F:mon.
+
+ Program Definition α := (sup (exist _ (iteres F) (iteres_directed F))).
+
+ Theorem Fixpoint_I_i : Fix F α -> is_least (Fix F) α.
+ Proof.
+ intro H. split; try assumption.
+  intros. apply sup_spec; cbn. intros z Q.
+  inversion Q. rewrite <- (itere_preserves_fix F y n).
+  now apply itere_monotony. assumption.
+ Qed.
+
+ Program Definition α' := (sup (exist _ (iteres_from_1 F) _)).
+ Next Obligation. apply iteres_from_1_directed. Qed.
+
+ Lemma sup_from_1 : α == α'.
+ Proof.
+  apply weq_spec. split. 
+  + apply sup_spec; cbn. intros. inversion H.
+  induction n. now cbn. apply leq_xsup.
+  apply from_bot_from_1. lia.
+  + apply sup_preserves_inclusion; cbn. apply from_1_included.
+ Qed.
+
+ Theorem Fixpoint_I_ii : Continuous F -> is_least (Fix F) α. (* Note that F is monotonous too. *)
+ Proof.
+  intro H.
+  assert (Fix F α).
+   + unfold Fix. destruct (H (iteres F) (iteres_directed F)) as [HD HS].
+    transitivity α'; try now rewrite sup_from_1. rewrite HS.
+    apply sup_is_independent_of_proof. cbn. unfold iff_part. apply image_of_iteres.
+   + now apply Fixpoint_I_i.
+ Qed.
+
+
+ (** * Fixpoint theorems and proofs : second theorem. *)
+
+ Lemma Induction_Rule : (exists µ0, is_least (Pre F) µ0)
+  -> exists µ, is_least (Fix F) µ /\ forall x, Pre F x -> µ <= x.
+ Proof.
+  intro H. destruct H as [µ0 Hmu0].
+  exists µ0. repeat split.
+  + apply weq_spec. split. apply Hmu0.
+    apply Hmu0. unfold Pre. apply Hbody. apply Hmu0.
+  + intros. apply Hmu0. now apply fix_is_pre.
+  + apply Hmu0.
+ Qed.
 
 Lemma P0_is_in_Post : included (P0 F) (Post F).
 Proof.
@@ -1022,600 +686,150 @@ Proof.
 Qed.
 (* Note : contrarily to the book, here P0' was never used for now, neither was phi. *)
 
-Definition down (x:X) := (fun z => z <= x).
-
-Lemma down_is_subCPO : forall x, is_subCPO (down x).
-Proof.
-  intros x D Hd. unfold down. apply sup_spec. intros. now apply Hd.
-Qed.
-
-Lemma P0_is_in_down x : Fix F x -> included (P0 F) (down x).
-Proof.
+ Lemma P0_is_in_down x : Fix F x -> included (P0 F) (down x).
+ Proof.
   intro. assert (Invariant F (down x) /\ is_subCPO (down x)).
   + split.
     - intros y Hy. inversion Hy. unfold down. rewrite <- H. apply Hbody. apply H0.
     - apply down_is_subCPO.
   + now apply P0_is_smallest_invariant_subCPO.
-Qed.
+ Qed.
 
-(* ------ sub-CPO ----- *)
-(* Define a set (part of X) as being a CPO *)
+ Program Instance P0_CPO : CPO (set_type (P0 F)) := (subCPO _).
+ Next Obligation. apply P0_is_invariant_subCPO. Qed.
 
-Definition set_type (Y : set X) : Type := { x : X | Y x}.
-Definition element Y (y :set_type Y) := proj1_sig y.
-
-Definition complete_body {Y : set X} (D : set (set_type Y)) : set X := 
-  (fun x => {is_in_Y : Y x & D (exist _ x is_in_Y)}).
-
-Check is_subCPO. Print is_subCPO.
-
-Program Definition subCPO (*{X} {P : CPO X}*) (Y:set X) (H : is_subCPO Y) : (CPO (set_type Y)) := {|
-   weq x y := (@weq X P) (element x) (element y);
-   leq x y := (@leq X P) (element x) (element y);
-   sup D := (@sup X P) (exist (Directed leq) (complete_body (Dbody D)) _) ;
- |}.
-Next Obligation. 
-  destruct D as [D Hd]. cbn. intros x y Hx Hy. inversion Hx. inversion Hy.
-  destruct (Hd (exist (fun x : X => Y x) x x0) (exist (fun x : X => Y x) y x1)) 
-    as [[z Pz] [Hz [Hxz Hyz]]]; try assumption.
-  exists z. split. now exists Pz. now split.
-Qed.
-Next Obligation.
-  apply H. intros x Hx.
-  destruct D as [D Hd]; cbn in Hx. now destruct Hx.
-Qed.
-Next Obligation.
-  apply Build_PreOrder; intro x. reflexivity. intros y z Hxy Hyz. now transitivity (element y).
-Qed.
-Next Obligation. apply weq_spec. Qed.
-Next Obligation. split.
-  + intros. apply (sup_spec (exist (Directed leq) (complete_body (Dbody D)) (subCPO_obligation_1 D))); cbn.
-    assumption. destruct y. cbn. now exists y.
-  + intros. apply sup_spec. cbn. intros. destruct H1. now apply (H0 (exist (fun x : X => Y x) y x)).
-Qed.
-
-Program Instance P0_CPO : CPO (set_type (P0 F)) := (subCPO _).
-Next Obligation. apply P0_is_invariant_subCPO. Qed.
-
-Program Definition G : @mon (set_type (P0 F)) P0_CPO := 
+ Program Definition F_restricted_to_P0 : @mon (set_type (P0 F)) P0_CPO := 
   {| body := fun y => (exist _ (F (element y)) _) |}.
-Next Obligation. destruct y as [x Hx]; cbn. apply P0_is_invariant_subCPO. now apply from_image. Qed.
-Next Obligation. intros y1 y2 H12; cbn. now apply Hbody. Qed.
+ Next Obligation. destruct y as [x Hx]; cbn. apply P0_is_invariant_subCPO. now apply from_image. Qed.
+ Next Obligation. intros y1 y2 H12; cbn. now apply Hbody. Qed.
 
-Lemma G_is_increasing : Increasing G.
-Proof. intro y. destruct y as [x Hx]; cbn. now apply P0_is_in_Post. Qed.
+ Lemma F_restricted_is_increasing : Increasing F_restricted_to_P0.
+ Proof. intro y. destruct y as [x Hx]; cbn. now apply P0_is_in_Post. Qed.
 
-Theorem Fixpoint_II : exists x, Fix F x.
-Proof.
-  destruct (increasing_has_fix_point G G_is_increasing).
+ Theorem Fixpoint_II : exists x, Fix F x.
+ Proof.
+  destruct (increasing_has_fix_point F_restricted_to_P0 F_restricted_is_increasing).
   destruct x as [x Hx]. cbn in H. now exists x.
-Qed.
+ Qed.
 
-(* Actually, we can go further. Since we constructively built the fixpoint of G as being (H_sup bot) for a well-chosen CPO.
-So we can define this fix-point and add the results from Claim 3 of the theorem : it is both the top of P0 and the least fixpoint of F.*)
+ (* Actually, we can go further. Since we constructively built the fixpoint of G as being (H_sup bot) for a well-chosen CPO.
+ So we can define this fixpoint and add the results from Claim 3 of the theorem : it is both the top of P0 and the least fixpoint of F.*)
 
-Definition a := (H_sup bot). (*Here a is of type (set_type P0) since this was the last CPO to be defined. 
-It's what we want, no need to specify implicit arguments. *) Check a.
-Print is_least.
+ Definition a := (H_sup bot). (*Here a is of type (set_type P0) since this was the last CPO to be defined. 
+ It's what we want, no need to specify implicit arguments. *)
 
-Lemma a_is_fixpoint_of_F : Fix F (element a).
-Proof.
-  assert (Fix G a). apply H_sup_bot_is_fix_point_of_all_Increasing. apply G_is_increasing.
+ Lemma a_is_fixpoint_of_F : Fix F (element a).
+ Proof.
+  assert (Fix F_restricted_to_P0 a). apply H_sup_bot_is_fixpoint_of_all_Increasing. apply F_restricted_is_increasing.
   destruct a as [a Ha]. now cbn in *.
-Qed.
+ Qed.
 
-Theorem a_is_top_of_P0_and_least_fixpoint_of_F : is_greatest (P0 F) (element a) /\ is_least (Fix F) (element a).
-Proof. split.
+ Theorem a_is_top_of_P0_and_least_fixpoint_of_F : is_greatest (P0 F) (element a) /\ is_least (Fix F) (element a).
+ Proof. split.
   + split. destruct a as [µ Hmu]. now cbn. apply P0_is_in_down.
    intros. apply a_is_fixpoint_of_F.
   + split. apply a_is_fixpoint_of_F. intros. apply (P0_is_in_down y).
     assumption. destruct a as [µ Hmu]. now cbn.
-Qed.
+ Qed.
+
+End Fixpoints.
 
 
 
-(* ------ Theorem III ------ *)
 
+(** * Theorem III : Bourbaki-Witt theorem. This theorem requires classic logic, it is false in intuitionist logic. *)
 
-(* Now show that P0 is a chain, to prove that it has a sup (top). *)
+Section Bourbaki_Witt.
 
-Definition Comparables (x:X) := (fun y => y <= x \/ x <= y).
+ Context {X} {P: CPO X}.
+ Definition classic_axiom := forall (P : Prop), P \/ ~ P.
 
-Definition lt {Y} {Q : CPO Y} x y := x <= y /\ ~ (x == y).
-Infix "<" := lt.
-Axiom classic : forall (P : Prop), P \/ ~ P.
+ (* Now show that P0 is a chain, to prove that it has a sup (top). This is a fixpoint. *)
 
-Definition A F' : set X := 
-  (fun x => (P0 F') x /\ forall y, (P0 F') y -> y < x -> F' y <= x).
+ Definition lt {Y} {Q : CPO Y} x y := x <= y /\ ~ (x == y).
+ Infix "<" := lt.
 
-Definition Ax F' x : set X :=
-  (fun y => (P0 F') y /\ (y <= x \/ F' x <= y)).
+ Lemma leq_is_lt_or_eq : classic_axiom -> forall x y, x <= y -> x==y \/ x < y. (* excluded middle ! *)
+ Proof. intros EM x y Hxy. destruct (EM (x==y)). now left. now right. Qed.
 
-Definition fun_ext (f:X->X) := Proper (weq ==> weq) f.
+ Lemma not_leq_and_gt : forall x y, ~ (x <= y /\ y < x). (* no need for EM *)
+ Proof. intros x y. intro. destruct H. destruct H0. contradict H1. now apply weq_spec. Qed.
 
+ Definition Extreme F' : set X := 
+  (fun c => (P0 F') c /\ forall x, (P0 F') x -> x < c -> F' x <= c).
 
-Axiom fun_ext_true : forall (f: X -> X), Proper (weq ==> weq) f. 
-(*temporary, I will give this as an hypothesis of lemmas that need it.*)
-
-Lemma Ax_are_invariant_subCPOs F' : Increasing F' -> forall x, A F' x 
-  -> Invariant F' (Ax F' x) /\ is_subCPO (Ax F' x).
-Proof.
-  intros HF x Ha. destruct Ha as [Px Hx]. split.
-  + intros y Hy. inversion Hy. split. apply P0_is_invariant_subCPO. apply from_image. apply H.
-    inversion H. destruct H2.
-    - destruct (classic (x <= x0)). (* WARNING : excluded middle here *)
-      right. apply weq_spec. apply fun_ext_true. (* WARNING :  functional extensionality here *)
-      now apply weq_spec.
-      left. apply (Hx x0). assumption. destruct (classic (x0 == x)). (* Warning : excluded middle here *)
-      contradict H3. apply weq_spec. apply H4. now split.
-     (*apply (Hx x0). destruct (Hx x0); intuition. right. now apply weq_spec.*)
-    - right. now transitivity x0.
-  + intros D Hi. assert (P0 F' (sup D)). apply P0_is_invariant_subCPO. transitivity (Ax F' x).
-    assumption. intros x0 Hx0. apply Hx0. split. apply H.
-    destruct (classic (exists y, (Dbody D) y /\ F' x <= y)). (* WARNING : excluded Middle here !!! *)
-    right. destruct H0 as [y Hy]. transitivity y. apply Hy. apply leq_xsup. apply Hy.
-    left. apply sup_spec. intros. destruct (Hi y). assumption.
-    destruct H3. assumption. contradict H0. now exists y.
-Qed.
-
-Lemma P0_is_Ax F' : Increasing F' -> forall x, (A F' x) -> (P0 F') == (Ax F' x).
-Proof.
-  intros HF x Hx. apply weq_spec. split.
-  + apply P0_is_smallest_invariant_subCPO. now apply Ax_are_invariant_subCPOs.
-    now apply Ax_are_invariant_subCPOs.
-  + intros y Hy. apply Hy.
-Qed.
-
-Lemma A_is_P0 F' : (Increasing F') -> (A F') == (P0 F').
-Proof. (*Lots and lots of excluded middle to manipulate "x < y" and 
-once to get : forall x, P x \/ Q x -> (exists x, Q x) \/ (forall x, P x). *)
-  intro HF. apply weq_spec. split.
-  + intros x Hx. apply Hx.
-  + apply P0_is_smallest_invariant_subCPO.
-    - intros x Hx. inversion Hx. split. apply P0_is_invariant_subCPO.
-      apply from_image. apply H.
-      intros. assert (Ax F' x0 y). apply P0_is_Ax; intuition. unfold Ax in H3.
-      destruct H3. destruct H4. destruct (classic (y < x0)).
-      transitivity x0. now apply H. apply HF. destruct (classic (y == x0)).
-      apply weq_spec. now apply fun_ext_true. contradict H4. intro. apply H5. now split.
-      destruct H2. contradict H5. now apply weq_spec.
-    - intros D HD. split. apply P0_is_invariant_subCPO. transitivity (A F').
-      assumption. intros x Hx. apply Hx.
-      intros y Hy Hs. 
-      destruct (classic (exists k, (Dbody D) k /\ y <= k)).
-      destruct H as [k [Dk Hyk]]. destruct (classic (y == k)).
-      assert (k < sup D). split. now apply leq_xsup. destruct Hs. now rewrite H in H1.
-      transitivity (F' k). apply weq_spec. now apply fun_ext_true.
-      assert (Ax F' k (sup D)). apply P0_is_Ax; intuition.
-      apply P0_is_invariant_subCPO. rewrite HD. intros x Hx. apply Hx.
-      destruct H1. destruct H2. destruct H0. contradict H3. now apply weq_spec.
-      assumption. transitivity k. destruct (HD k Dk). now apply (H1 y). 
-      now apply leq_xsup.
-      assert (sup D <= y). apply sup_spec. intros. destruct (classic (y == y0)).
-      now apply weq_spec. destruct (classic (y0 <= y)). assumption. contradict H.
-      exists y0. split. assumption. assert (Ax F' y0 y). apply P0_is_Ax; intuition.
-      destruct H. destruct H3; intuition. contradict H2. rewrite <- H3. apply HF.
-      destruct Hs. contradict H2. now apply weq_spec.
-Qed.
-
-(*
-Program Definition G' (F': X -> X) : set_type (P0 F') -> set_type (P0 F') := 
-  fun x => (exist _ (F' (element x)) _).
-Next Obligation.
-destruct x as [x Hx]; cbn. apply P0_is_invariant_subCPO. now apply from_image. Qed.
-*)
-
-Definition is_Chain (Y : set X) := forall (x y : X), Y x -> Y y -> x <= y \/ y <= x.
-
-Lemma P0_is_Chain (F':X -> X) : Increasing F' -> is_Chain (P0 F').
-Proof.
-  intros HF x y Hx Hy. assert (Ax F' x y).
-  apply P0_is_Ax; intuition. now prew (A_is_P0 HF).
-  destruct H. destruct H0. now right. left. transitivity (F' x).
-  apply HF. assumption.
-Qed.
-
-Lemma chain_is_directed {Y} {Q : CPO Y} : forall D, is_Chain D -> Directed leq D.
-Proof.
-  intros D Hd x y Hx Hy. destruct (Hd x y); intuition.
-  exists y. now split.
-  exists x. now split.
-Qed.
-
-Lemma P0_is_directed (F':X -> X) : Increasing F' -> Directed leq (P0 F').
-Proof. intro HF. apply chain_is_directed. now apply P0_is_Chain. Qed.
-
-Program Definition top_P0 (F':X -> X) (H : Increasing F') := (sup (exist _ (P0 F') _)).
-Next Obligation. apply P0_is_directed. apply H. Qed.
-
-Definition is_minimal {Y} {Q : CPO Y} S x := S x /\ forall y, S y -> y <= x -> y == x.
-
-(*The book is wrong : the top of P0 is not necessarily minimal (cf counterexample on paper)
-However, from an existing fix point, it seems we can deduce a minimal fix point since the set of 
-fixpoints between bottom and our fix point is a chain.*)
-Theorem Fixpoint_III (F' : X -> X) : Increasing F' -> exists x, Fix F' x(*is_minimal (Fix F') x*).
-Proof.
-  intro HF. exists (top_P0 HF). (* split.
-  +*) apply weq_spec. split. apply leq_xsup; cbn. apply P0_is_invariant_subCPO.
-   apply from_image. apply P0_is_invariant_subCPO; cbn. intro. now intro.
-   apply sup_spec; cbn. intros. transitivity (top_P0 HF). now apply leq_xsup.
-   apply HF.
-Qed.
-
-
-(* ------------------ Another approah, trying to avoid excluded middle ----------------------- *)
-
-(* Found an article stating that this theorem is False in intuitionist logic ! *)
-(* TODO : clean up above proof using classical logic, or make it clean below using Bourbaki's proof.
-State that x <= y -> ... and same with the set D that is all below x or has an element above x *)
-
-(* with ordinals ?*)
-Inductive C (F' : X -> X) : set X := 
-  | C_bot : C F' bot
-  | C_succ : forall x, C F' x -> C F' (F' x)
-  | C_lim : forall D, included (Dbody D) (C F') -> C F' (sup D).
-
-(* Now we want to prove that C is a chain. Note that C = P0' = P0, hence the proofs above. *)
-
-
-
-Definition Extreme F' : set X := 
-  (fun c => (P0 F') c /\ forall x, (P0 F') x -> x <= c -> x==c \/ F' x <= c).
-
-Definition Mc F' c : set X :=
+ Definition Mc F' c : set X :=
   (fun x => (P0 F') x /\ (x <= c \/ F' c <= x)).
 
-Lemma Mc_is_P0 F' : Increasing F' -> forall c, Extreme F' c -> (P0 F') == (Mc F' c).
-Proof.
-  intros HF c Ec. destruct Ec as [Pc Ec']. split.
+ Lemma Mc_is_P0 F' : classic_axiom -> (Proper (weq ==> weq) F') -> Increasing F' -> forall c, Extreme F' c -> iff_part (P0 F') (Mc F' c).
+ Proof.
+  intros EM Fp HF c Ec. destruct Ec as [Pc Ec']. split.
   + apply P0_is_smallest_invariant_subCPO.
     - intros x Hx. inversion Hx. split. apply P0_is_invariant_subCPO. apply from_image. apply H.
       destruct H as [Px0 Hx0]. destruct Hx0.
-      * destruct (Ec' x0); intuition. right. apply weq_spec. now apply fun_ext_true.
+      * apply leq_is_lt_or_eq in H. destruct H. right. apply weq_spec. now apply Fp.
+        left. now apply Ec'. assumption.
       * right. transitivity x0. assumption. apply HF.
     - intros D Hi. split. 
       apply P0_is_invariant_subCPO. rewrite Hi. intros x0 Hx0. apply Hx0.
-      destruct (classic (exists y, (Dbody D) y /\ F' c <= y)). (* WARNING : excluded Middle here !!! *)
-      right. destruct H as [y Hy]. transitivity y. apply Hy. now apply leq_xsup.
-      left. apply sup_spec. intros. destruct (Hi y). assumption.
-      destruct H2. assumption. contradict H. now exists y. (* Need excluded middle to prove subCPO here :'( *)
+      destruct (EM (exists y, (Dbody D) y /\ F' c <= y)). (* WARNING : excluded middle ! *)
+      * right. destruct H as [y Hy]. transitivity y. apply Hy. now apply leq_xsup.
+      * left. apply sup_spec. intros. destruct (Hi y). assumption.
+        destruct H2. assumption. contradict H. now exists y.
   + intro Hm. apply Hm.
-Qed.
+ Qed.
 
-Lemma P0_is_extreme F' : Increasing F' -> forall x, P0 F' x -> Extreme F' x.
-Proof.
-  intros HF. apply P0_is_smallest_invariant_subCPO.
-  +  intros c Hc. inversion Hc. inversion H as [HPx HEx]. split.
+ Lemma P0_is_extreme F' : classic_axiom -> (Proper (weq ==> weq) F') ->  Increasing F' -> forall x, P0 F' x -> Extreme F' x.
+ Proof.
+  intros EM Fp HF. apply P0_is_smallest_invariant_subCPO.
+  + intros c Hc. inversion Hc. inversion H as [HPx HEx]. split.
     - apply P0_is_invariant_subCPO. now apply from_image.
-    - intros. assert (P0 F' == Mc F' x). apply (Mc_is_P0 HF H). 
-    assert (Mc F' x x0). now rewrite <- (set_eq H3 x0).
-    destruct H4. destruct H5.
-    
-     destruct (classic (x0 == F' x)). now left. (* WARNING : another excluded middle here *)
-      right.
-      (*TODO : finish *)
-Admitted.
-
-
-
-
-
-
-
-
-
-
-
-End fixpoint.
-
-
-
-
-
-(* ------------------------  END OF CURRENT WORK ------------------------------ *)
-
-
-
-
-
-
-
-
-
-
-
-
-
-
-
-
-
-
-
-
-
-
-
-
-
-
-
-
-
-
-
- 
-
-(** * Concrete instances *)
-
-(** Prop is a complete lattice *)
-Program Instance CompleteLattice_Prop: CompleteLattice Prop :=
-  {| weq:=iff;
-     leq:=Basics.impl;
-     sup Y:=exists2 P, Y P & P;
-  |}.
-Next Obligation. firstorder. Qed.
-Next Obligation. firstorder. Qed.
-
-(** Functions into a complete lattice form a complete lattice *)
-Program Instance CompleteLattice_fun {A X} {L: CompleteLattice X}: CompleteLattice (A -> X) :=
-  {| weq:=pointwise_relation A weq;
-     leq:=pointwise_relation A leq;
-     sup F a:=sup (fun b => exists2 f, F f & b=f a);
-  |}.
-Next Obligation. 
-  constructor.
-   now intros f x. 
-   intros f g h H H' x. now transitivity (g x).
-Qed.
-Next Obligation. unfold pointwise_relation. setoid_rewrite weq_spec. firstorder. Qed.
-Next Obligation.
-  unfold pointwise_relation. setoid_rewrite sup_spec.
-  firstorder. rewrite H1. now apply H. 
-Qed.
-
-
-
-
-(** * The complete lattice of monotone endofunctions *)
-
-Section mon. 
- Context {X} {L: CompleteLattice X}.
- 
- (** monotone endofunctions *)
- Record mon := { body:> X -> X; Hbody: Proper (leq ==> leq) body }.
- 
- (** the following instances are not global: more powerful ones are 
-    given at the end of the section *)
- Existing Instance Hbody.
- Instance Hbody' (f: mon): Proper (weq ==> weq) f.
- Proof. intros x y. rewrite 2weq_spec. now split; apply f. Qed.
-
- (** constant function *)
- Program Definition const x: mon := {| body y := x |}.
- Next Obligation. intros ? ? ?. reflexivity. Qed.
-
- (** identity and composition
-     the monotonicity proofs are transparent to get strong equalities
-     - [id ° f = f ° id = f], and
-     - [f ° (g ° h) = (f ° g) ° h]
-  *)
- Definition id: mon := {| 
-   body x := x; 
-   Hbody x y H := H 
- |}.
-
- Definition comp (f g: mon): mon := {|
-   body := fun x => f (g x); 
-   Hbody x y H := Hbody f _ _ (Hbody g _ _ H) 
- |}.
- Infix "°" := comp (at level 20): lattice.
- 
- (** monotone endofunctions form a new complete lattice *)
- Global Program Instance CompleteLattice_mon: CompleteLattice mon := {|
-   weq := pointwise_relation X weq;
-   leq := pointwise_relation X leq;
-   sup F := {| body a := sup (fun b => exists2 f, F f & b=f a) |};
- |}.
- Next Obligation.
-   intros x y H. apply sup_spec. intros i [f Ff ->].
-   rewrite H. apply leq_xsup. eauto. 
- Qed.
- Next Obligation. constructor. now intros f x. intros f g h H H' x. now transitivity (g x). Qed.
- Next Obligation. unfold pointwise_relation. setoid_rewrite weq_spec. firstorder. Qed.
- Next Obligation.
-   unfold pointwise_relation. setoid_rewrite sup_spec.
-   firstorder. rewrite H1. auto. 
+    - intros. assert (iff_part (P0 F') (Mc F' x)). apply (Mc_is_P0 EM Fp HF H).
+      assert (Mc F' x x0). now rewrite <- (set_eq H3 x0). destruct H4. destruct H5.
+      * apply leq_is_lt_or_eq in H5; intuition.
+        apply weq_spec. now apply Fp. transitivity x; intuition.
+      * exfalso. eapply not_leq_and_gt. split. apply H5. apply H2.
+  + intros D Ed. split. apply P0_is_invariant_subCPO. rewrite Ed. intros x Hx. apply Hx.
+    intros x Px Hxd. destruct (EM (exists c, (Dbody D) c /\ x <= c)).
+    - destruct H as [c [Hdc Hcx]]. apply leq_is_lt_or_eq in Hcx; intuition.
+      * transitivity (F' c). apply weq_spec. now apply Fp.
+        assert (Mc F' c (sup D)). apply Mc_is_P0; intuition. apply P0_is_invariant_subCPO.
+          rewrite Ed. intros y Hy. apply Hy.
+        destruct H0. destruct H1. exfalso. eapply not_leq_and_gt. split. rewrite <- H in H1.
+        apply H1. apply Hxd. assumption.
+      * transitivity c. apply Ed; intuition. now apply leq_xsup.
+    - assert (sup D <= x).
+      * apply sup_spec. intros. rewrite HF. assert (Mc F' y x). apply Mc_is_P0; intuition.
+        destruct H1. destruct H2. contradict H. now exists y. assumption.
+      * exfalso. eapply not_leq_and_gt. split. apply H0. assumption.
  Qed.
 
- Global Instance comp_leq: Proper (leq ==> leq ==> leq) comp.
- Proof. intros f f' Hf g g' Hg x. simpl. rewrite (Hg x). apply Hf. Qed.
- Global Instance comp_weq: Proper (weq ==> weq ==> weq) comp := op_leq_weq_2.
 
- Lemma compA f g h: f ° (g ° h) = (f ° g) ° h.
- Proof. reflexivity. Qed.
- Lemma compIx f: id ° f = f.
- Proof. now case f. Qed. 
- Lemma compxI f: f ° id = f.
- Proof. now case f. Qed. 
+ Lemma P0_is_Chain (F':X -> X) : classic_axiom -> (Proper (weq ==> weq) F') -> Increasing F' -> is_Chain (P0 F').
+ Proof.
+  intros EM Fp HF x y Hx Hy. assert (Mc F' x y).
+  apply Mc_is_P0; intuition. apply P0_is_extreme; intuition.
+  destruct H. destruct H0. now right. left. transitivity (F' x).
+  apply HF. assumption.
+ Qed.
 
-End mon.
-Arguments mon X {L}.
-Infix "°" := comp (at level 20): lattice.
+ Lemma P0_is_directed (F':X -> X) : classic_axiom -> (Proper (weq ==> weq) F') -> Increasing F' -> Directed leq (P0 F').
+ Proof. intros EM Fp HF. apply chain_is_directed. now apply P0_is_Chain. Qed.
 
-(** application as a function [X->X]->X->X is monotone in its two arguments *)
-Instance app_leq {X} {L: CompleteLattice X}: Proper (leq ==> leq ==> leq) body.
-Proof. intros f g fg x y xy. transitivity (f y). now apply f. now apply fg. Qed.
-Instance app_weq {X} {L: CompleteLattice X}: Proper (weq ==> weq ==> weq) body := op_leq_weq_2.
+(* Note : since we put excluded middle and functional extensionality as hypothesis, we lose constructivity,
+we can't just define our fixpoint as below :
+Program Definition top_P0 (F':X -> X) (H : Increasing F') := (sup (exist _ (P0 F') _)).
+Next Obligation. apply P0_is_directed; intuition. apply H. Qed. *)
 
+(*The book is wrong : the top of P0 is not necessarily minimal (cf counterexample on paper)
+However, from an existing fix point, it seems we can deduce a minimal fix point since the set of 
+fixpoints between bottom and our fix point is a chain. TODO ? *)
+ Theorem Fixpoint_III (F' : X -> X) : classic_axiom -> (Proper (weq ==> weq) F') -> Increasing F' -> exists x, Fix F' x(*is_minimal (Fix F') x*).
+ Proof.
+  intros EM Fp HF. exists (sup (exist _ (P0 F') (P0_is_directed EM Fp HF))).
+  apply weq_spec. split. apply leq_xsup; cbn. apply P0_is_invariant_subCPO.
+  apply from_image. apply P0_is_invariant_subCPO; cbn. intro. now intro.
+  apply sup_spec; cbn. intros. rewrite <- HF. now apply leq_xsup.
+ Qed.
 
-
-(** * Compatibility *)
-
- (** ** compatible functions *)
- Notation compat f := (f ° b <= b ° f) (only parsing).
- 
- (** compositionality properties of compatibility *)
- Lemma compat_id: compat id.
-Proof. reflexivity. Qed.
- 
- Lemma compat_comp f g: compat f -> compat g -> compat (f ° g).
-Proof. intros H1 H2. rewrite compA. rewrite <- H1. rewrite <- !compA. rewrite H2. reflexivity. Qed.
-
- Lemma compat_b: compat b.
-Proof. reflexivity. Qed.
-
- Lemma compat_const y: y <= b y -> compat (const y).
-Proof. intro H. intro x. simpl. apply H. Qed.
- 
- Lemma compat_sup (F: mon X -> Prop):
-   (forall f, F f -> compat f) -> compat (sup F).
-Proof. intros H x. simpl. rewrite sup_spec. intros y Q. destruct Q as [f Q1 Q2].
-  rewrite Q2. (* ici rewrite (H f). ne marche pas car il semble incapable de reconnaitre f (b x)*)
-  assert (f (b x) = (f ° b) x).
-    + simpl. reflexivity.
-    + rewrite H0. rewrite (H f). (* je peux enfin le faire ! *)
-      - simpl. apply Hbody. rewrite -> (leq_xsup (fun b0 : X => exists2 f0 : mon X, F f0 & b0 = f0 x)).
-        reflexivity. exists f. apply Q1. reflexivity.
-      - apply Q1.
-Qed.
-
-
- (** compatible closures provide upto techniques *)
- Proposition upto f:
-   compat f -> id <= f -> f ° f <= f ->
-   forall x, x <= b (f x) -> x <= gfp.
-Proof.
-  intros H1 H2 H3 x H5. transitivity (f(x)). apply H2.
-  apply leq_gfp. rewrite H5 at 1.
-  assert (f (b (f x)) = (f ° b) (f x)). easy.
-  rewrite H. rewrite H1.
-  assert ((b ° f) (f x) = (b ° (f ° f)) x). easy.
-  rewrite H0. rewrite H3. reflexivity.
-Qed.
-
-(** * Companion *)
-
- (** the companion is the largest compatible function *)
- Definition t := sup (fun f => compat f).
-
- Lemma compat_t: compat t.
- Proof. now apply compat_sup. Qed.
-
- (** more properties about [t] *)
- Lemma leq_t: forall f, compat f -> f <= t.
- Proof. apply leq_xsup. Qed.
- 
- Lemma id_t: id <= t.
-Proof. apply leq_t. reflexivity. Qed.
-
- Lemma b_t: b <= t.
-Proof. apply leq_t. apply compat_b. Qed.
-
- Lemma tt_t: t ° t <= t.
-Proof. apply leq_t.
-  rewrite compA. rewrite <- compat_t. rewrite <- !compA. rewrite compat_t. reflexivity.
-Qed.
-
- Lemma t_idem: t ° t == t.
-Proof.
-  rewrite weq_spec. split. apply tt_t.
-  assert ((id°t) <= t ° t). rewrite id_t. reflexivity. rewrite <- H. reflexivity.
-Qed.
-
- (** enhanced coinduction principle *)
- Definition bt := b ° t.
- Lemma coinduction x: x <= bt x -> x <= gfp.
-Proof.
-  intro H. apply upto with t.
-  + apply compat_t.
-  + apply id_t.
-  + apply tt_t.
-  + apply H.
-Qed.
-
-
- (** characterisation of the greatest fixpoint via the companion *)
- Proposition gfp_tbot : gfp == t bot.
-apply from_above. intro. split.
-  + intro. apply sup_spec. intros. destruct H0 as [f ? ?]. rewrite <- H. apply leq_gfp.
-    rewrite H1. assert ((b (f bot)) =(b ° f) bot). easy. rewrite H2. rewrite <- H0. simpl.
-    apply Hbody. easy.
-  + intro H. apply sup_spec. intros y H0. rewrite <- H. apply leq_xsup. exists (const y).
-    - apply compat_const. apply H0.
-    - simpl. reflexivity.
-Qed.
- 
- (** to sum up: [gfp = t bot = t gfp <= t x] *)
- Corollary t_gfp: t gfp == gfp.
-Proof. 
-  rewrite weq_spec. split.
-  + rewrite gfp_tbot at 1. assert (t (t bot) = (t ° t) bot) as H0. easy.
-   rewrite H0. rewrite tt_t. rewrite gfp_tbot. reflexivity.
-  + assert ((t bot) <= (t gfp)). apply Hbody. easy. rewrite gfp_tbot at 1. apply H.
-Qed.
-
- Corollary gfp_t x: gfp <= t x.
-Proof.
-  transitivity (t bot). rewrite gfp_tbot. reflexivity.
-  apply Hbody. easy.
-Qed.
-
-
-
-
-
-(* Homework questions to do on paper or in Coq*)
-
-
-(* Q1. Prove existence of a least fix point*)
-
- Definition lfp := inf (fun x => b x <= x). (*this will be proven a least fix point*)
-
- Lemma leq_xinf (P: X -> Prop) y: P y -> inf P <= y.
- Proof. now apply inf_spec. Qed.
-
- Proposition leq_lfp: forall y, b y <= y -> lfp <= y.  (*thus all fix points are greater than lfp*)
- Proof. apply leq_xinf. Qed.
-
- Lemma lfp_pfp:  b lfp <= lfp.
-Proof.
-  apply inf_spec. intros y H. rewrite <- H. apply Hbody.
-  apply leq_xinf. apply H.
-Qed.
-
- Lemma lfp_fp: lfp == b lfp. (*and lfp is indeed a fixpoint. CQFD Q1.*)
-Proof.
-  rewrite weq_spec. split.
-  + apply leq_xinf. apply Hbody. apply lfp_pfp.
-  + apply lfp_pfp.
-Qed.
-
-
-
-(* Q2. Prove compatibility of f\/g from compatibility of f and g.*)
-Lemma cup_comp f g h: cup f g ° h == cup (f ° h) (g ° h). Admitted.
-
-Lemma cup_preserve (z : mon X) (t : mon X) : forall (x : mon X) (y : mon X), x <= z -> y <= t -> cup x y <= (cup z t).
-Proof.
-  intros x y H Q. apply cup_spec. split.
-  + rewrite H. apply leq_xsup. left. reflexivity.
-  + rewrite Q. apply leq_xsup. right. reflexivity.
-Qed.
-
-Lemma meet_compat : forall f g, compat f -> compat g -> compat (cup f g).
-Proof.
-  intros. rewrite cup_comp. rewrite (cup_preserve H H0). rewrite cup_spec. split.
-  + assert (f <= cup f g). - apply leq_xsup. left. reflexivity. 
-    - rewrite <- H1. reflexivity.
-  + assert (g <= cup f g). - apply leq_xsup. right. reflexivity. 
-    - rewrite <- H1. reflexivity.
-Qed.
-
-
-
-
-
-
-
-
+End Bourbaki_Witt.
